finish fsub/autosubst2 typing_subst

fsub/autosubst2_dctx/prop_typing.v
@@ -1,6 +1,114 @@
+Require Import List.
+Require Import Program.Equality.
+From Hammer Require Import Tactics.
+From Coq Require Import ssreflect ssrfun ssrbool.
+
 Require Import common.prop_as_core.
 Require Import common.prop_as_unscoped.
 Require Import fsub.autosubst2_dctx.def_as2.
 Require Import fsub.autosubst2_dctx.def_extra.
 Require Import fsub.autosubst2_dctx.prop_basic.
 Require Import fsub.autosubst2_dctx.prop_subtyping.
+
+Import SubstNotations.
+Import UnscopedNotations.
+
+Lemma typing_narrowing Δ1 Δ2 Γ A B C t :
+  Δ2 ++ A :: Δ1 ;; Γ ⊢ t : C ->
+  Δ1 ⊢ B <: A ->
+  Δ2 ++ B :: Δ1 ;; Γ ⊢ t : C.
+Proof.
+  intro H. dependent induction H; intros; 
+    try hauto ctrs:typing.
+  - apply typing_abs.
+    + eapply wf_typ_narrowing; eauto.
+    + eauto.
+  - apply typing_tabs; eauto.
+    + eapply wf_typ_narrowing; eauto.
+    + replace (A0 :: Δ2 ++ B :: Δ1) with ((A0 :: Δ2) ++ B :: Δ1) by auto.
+      eapply IHtyping; simpl; eauto. 
+  - eapply typing_tapp; eauto using subtyping_narrowing.
+  - eapply typing_sub; eauto using subtyping_narrowing.
+Qed.
+
+Definition ctx_var_subst Δ Γ Γ' σ τ :=
+  forall x A, lookup_var x Γ A -> (Δ ;; Γ' ⊢ τ x : A [σ]).
+
+Lemma typing_subst Δ Δ' Γ Γ' A t σ τ :
+  Δ ;; Γ ⊢ t : A ->
+  ctx_tvar_subst Δ Δ' σ ->
+  ctx_var_subst Δ' Γ Γ' σ τ -> 
+  Δ' ;; Γ' ⊢ t [σ;τ] : A [σ] .
+Proof.
+  move => Hty. move : Δ' Γ' σ τ.
+  induction Hty; intros; asimpl; try hauto ctrs:typing.
+  - eapply typing_abs; eauto. 
+    + hauto unfold:ctx_tvar_subst_wf,ctx_tvar_subst use:wf_typ_subst_tvar,sub_wf_typ1.
+    + eapply IHHty; eauto.
+      * unfold ctx_var_subst in *. intros.
+        inversion H2; subst; asimpl; eauto.
+        -- hauto ctrs:lookup_var, typing.
+        -- eapply typing_weakening_var0; eauto. 
+  - eapply typing_tabs.
+    + hauto unfold:ctx_tvar_subst_wf,ctx_tvar_subst use:wf_typ_subst_tvar,sub_wf_typ1.
+    + eapply IHHty; eauto.
+      * unfold ctx_tvar_subst in *. intros.
+        inversion H2; subst; asimpl; eauto.
+        eapply sub_tvar_bound; try hauto ctrs:lookup_tvar use:subtyping_reflexivity simp+:asimpl.
+        asimpl. apply subtyping_reflexivity. eapply wf_typ_subst_tvar; eauto. 
+        -- hauto unfold:ctx_tvar_subst_wf ctrs:lookup_tvar use:wf_typ_weakening_tvar0,sub_wf_typ1,sub_wf_typ2. 
+        -- replace ( subst_typ (σ >> ren_typ ↑) A1) with (A1 [σ] ⟨ ↑ ⟩) by (asimpl; auto).
+           replace ( (σ >> ren_typ ↑) n) with ((σ n) ⟨ ↑ ⟩) by (asimpl; auto).
+           eapply sub_weakening_tvar0; eauto.
+      * unfold ctx_var_subst in *. intros.
+        apply lookup_var_map_inv in H2. ssimpl. asimpl.
+        replace (subst_typ (σ >> ren_typ ↑) A1) with (A1 [σ] ⟨ ↑ ⟩) by (asimpl; auto).
+        eapply typing_weakening_tvar0. eapply H1; eauto.
+  - asimpl. subst.
+    eapply typing_tapp with (A:=A [σ]) (B:=B [up_typ_typ σ]); asimpl; eauto. 
+    eapply subtyping_subst; eauto.
+  - eapply typing_sub with (A:=A [σ]); eauto.
+    eapply subtyping_subst; eauto.
+Qed.
+
+Definition wf_ctx Δ :=
+  forall X A, lookup_tvar X Δ A -> Δ ⊢ A.
+
+Lemma typing_abs_inv Δ Γ A A' B C t :
+  Δ ;; Γ ⊢ exp_abs A t : B ->
+  Δ ⊢ B <: typ_arr A' C ->
+  ((Δ ⊢ A' <: A) /\ (exists C', (Δ ;; (A :: Γ) ⊢ t : C') /\ (Δ ⊢ C' <: C))).
+Proof.
+  move => H. move : C A'. dependent induction H; intros; try hauto ctrs:typing.
+  - inversion H1; eauto.
+  - eapply IHtyping; eauto.
+    eapply subtyping_transitivity; eauto.
+Qed.
+
+Lemma typing_tabs_inv Δ Γ A A' B C t :
+  Δ ;; Γ ⊢ exp_tabs A t : B ->
+  Δ ⊢ B <: typ_all A' C ->
+  ((Δ ⊢ A' <: A) /\ (exists C', ((A'::Δ) ;; (map (ren_typ ↑) Γ) ⊢ t : C') /\ (A'::Δ ⊢ C' <: C))).
+Proof.
+  move => H. move : C A'. dependent induction H; intros; try hauto ctrs:typing.
+  - inversion H1; subst; split; eauto. eexists; split; eauto.
+    eapply (typing_narrowing _ nil); eauto.
+  - eauto using subtyping_transitivity.
+Qed.
+
+Theorem preservation Δ Γ t A t' :
+  Δ ;; Γ ⊢ t : A ->
+  wf_ctx Δ ->
+  t ⤳ t' ->
+  Δ ;; Γ ⊢ t' : A.
+Proof.
+  move => Hty Hwf Hstep. move : Δ Γ A Hty Hwf.
+  induction Hstep; intros; eauto using typing;
+    dependent induction Hty; try hauto ctrs:typing.
+  - inversion Hty1; subst.
+    + admit.
+    + eapply typing_abs_inv in H1; eauto. admit. 
+  - inversion Hty; subst.
+    + admit.
+    + eapply typing_tabs_inv in H1; eauto.
+Admitted.
